src/Domains/Sign_Side_Soundness.thy
@@ -11,7 +11,6 @@ theorem side_sign_analysis_sound:
     "t \<in> cfg_collect (to_cfg c) {s} (cfg_exit (to_cfg c))"
   assumes side_solve_dom:
     "side_cfg_solve_dom (to_cfg c) sign_tf bot s0 (cfg_exit (to_cfg c))"
-  assumes s0_global_bot: "restrict_global s0 = bot"
   shows "t \<in> sign_domain.gamma_state
        (side_analyse c sign_tf bot s0 (cfg_exit (to_cfg c)))"
 proof -
@@ -20,7 +19,7 @@ proof -
     "cfg_path (to_cfg c) (cfg_entry (to_cfg c)) es (cfg_exit (to_cfg c))"
     using runs_to_imp_path[OF exit_in_collect[folded runs_to_def]] by blast
   show ?thesis
-    by (smt (verit, del_insts) ep exit_in_collect fin s0_global_bot s_sound side_solve_dom
+    by (smt (verit, del_insts) ep exit_in_collect fin s_sound side_solve_dom
         sign_domain.sound_domain_axioms sign_sound_tf.sound_transfer_axioms sign_tf_mono
         sound_domain.side_solver_sound sound_transfer.tf_sound_assign sound_transfer.tf_sound_assume
         sound_transfer.tf_sound_assume_not sound_transfer.tf_sound_enter)
